:PROPERTIES:
:ID:       80120a64-eeb7-471c-94e2-a3c537a21699
:END:
#+title: Laplace Transform
#+date: [2024-09-08 Sun 16:06]
#+AUTHOR: Baley Eccles - 652137
#+STARTUP: latexpreview

* Laplace Transform
 - Uses [[id:d2083e8a-7a7a-48a8-89f4-9d13bba76b50][Transform Theory]] to convert signals into
 - Useful for

** Definition
 - \[F(s)=\int_{-\infty}^{\infty}f(t)e^{-st}dt\]
 - \[F(s)=\mathcal{L}\{f(t)\}\]
 - \[s=\sigma + i\omega\]
** Inverse
 - \[y(t)=\frac{1}{2\pi j}\int_{\sigma-j\infty}^{\sigma+j\infty}Y(s)e^{st}ds\]
   - This is hard to use

** Things
 - if \[f(t)=\delta(t-\tau)\]
   - then \[F(s)=e^{-s\tau}\]
 - if \[f(t)=u(t)\]
   - then \[F(s)=\frac{1}{s} \textrm{, for } \sigma>0\]
** Laplace to [[id:e2fd0b83-635c-48b4-85c0-2067477a0e63][Fourier Transform]]
 - This can only work one way, Laplace to Fourier
 - when \[s=j\omega \Rightarrow \sigma=0\]
 - There is one exception for this
   - when \[f(t)=u(t)\]
** Properties
 - Linearality:
   - \[a_1x_1(t)+a_2x_2(t)\leftrightarrow a_1X_1(s)+a_2X_2(s)\]
 - Time-shifting:
   - \[x(t-\tau) \leftrightarrow e^{-s\tau}X(s)\]
 - S-domain shifting:
   - \[e^{s_0t}x(t) \leftrightarrow X(s-s_0)\]
 - Scaling in time:
   - \[x(at) \leftrightarrow \frac{1}{\lvert a\rvert}X(\frac{s}{a})\]
 - Time reversal:
   - \[x(-t) \leftrightarrow X(-s)\]
 - Differentiation (t)
   - \[\frac{dx(t)}{dt} \leftrightarrow sX(s)\]
 - Differentiation (s):
   - \[tx(t) \leftrightarrow -\frac{dX(s)}{ds}\]
 - Convolution
   - \[x_1(t)*x_2(t) \leftrightarrow X_1(s)X_2(s)\]
 - Integration
   - \[\int_{-\infty}^tx(\lambda)d\lambda \leftrightarrow \frac{x(s)}{s}\]

** Partial Fraction Expansion
*** Example 1
\begin{align*}
Y(s)&=\frac{1}{(s+3)(s+1)} \\
Y(s)&=\frac{A}{s+3}+\frac{B}{s+1} \\
\Rightarrow 1&=A(s+1)+B(s+3) \\
\textrm{let } s=-1, 1&=A(0)+B(-1+3) \\
\Rightarrow B&=\frac{1}{2} \\
\Rightarrow A&=\frac{-1}{2}
\end{align*}
*** Example 2
- Quadratic factor in denominator
  - Linear factor in numerator
\begin{align*}
X(s)&=\frac{s+1}{s(s^2+9)} \\
\frac{s+1}{s(s^2+9)}&=\frac{A}{s}+\frac{Bs+c}{S^2+9} \\
\Rightarrow s+1&=A(s^2+9)+s(Bs+c) \\
\textrm{let } s=0, 1&=9A \Rightarrow A=\frac{1}{9} \\
\textrm{let } s=-1, 0&=10\frac{1}{9}+B-c \\
\textrm{let } s=1, 2&=A10+B-c \\
\Rightarrow B&=-\frac{1}{9} \\
\Rightarrow C&=1
\end{align*}
 - This will typically involve sin and cos terms.
